@prefix brick: <https://brickschema.org/schema/Brick#> .
@prefix occ: <https://brickschema.org/schema/Brick/extension/occupancy#> .
@prefix sh: <http://www.w3.org/ns/shacl#> .
@prefix owl: <http://www.w3.org/2002/07/owl#> .
@prefix rdf: <http://www.w3.org/1999/02/22-rdf-syntax-ns#> .
@prefix rdfs: <http://www.w3.org/2000/01/rdf-schema#> .
@prefix skos: <http://www.w3.org/2004/02/skos/core#> .
@prefix foaf: <http://xmlns.com/foaf/0.1/> .
@prefix sdo: <http://schema.org/> .
@prefix dcterms: <http://purl.org/dc/terms#> .
@prefix unit: <http://qudt.org/vocab/unit/> .
@prefix qudt: <http://qudt.org/schema/qudt/> .
@prefix qkdv: <http://qudt.org/vocab/dimensionvector/> .
@prefix quantitykind: <http://qudt.org/vocab/quantitykind/> .
@prefix xsd: <http://www.w3.org/2001/XMLSchema#> .

occ: a owl:Ontology ;
    rdfs:label "Brick Occupancy Ontology" ;
    dcterms:creator ( [ a sdo:Person ;
                sdo:email "gtfierro@cs.berkeley.edu" ;
                sdo:name "Gabe Fierro" ] ) ;
    dcterms:license <https://github.com/BrickSchema/brick/blob/master/LICENSE> ;
    rdfs:seeAlso <https://brickschema.org> .



occ:label   rdfs:subPropertyOf  rdfs:label ;
    skos:definition "The name or identifier or other label for this entity" ;
    rdfs:domain xsd:string  ;
.

occ:hasAssignedLocation a   owl:ObjectProperty ;
    owl:inverseOf   occ:isAssignedLocationOf ;
    rdfs:subPropertyOf  brick:hasLocation ;
    rdfs:domain occ:Occupant ;
    skos:definition "Occupant is assigned to, or otherwise habitually or nominally occupies the indicated Location" ;
.

occ:isAssignedLocationOf    a   owl:ObjectProperty ;
    owl:inverseOf   occ:isAssignedLocationOf ;
    rdfs:subPropertyOf  brick:isLocationOf ;
    rdfs:domain brick:Location ;
    skos:definition "Location is assigned to, or otherwise habitually or nominally occupied by the indicated Occupant" ;
.


occ:hasAccessTo    a   owl:ObjectProperty ;
    sh:class    brick:Equipment ;
    owl:inverseOf   occ:isAccessibleBy ;
.

occ:isAccessibleBy  a   owl:ObjectProperty ;
    sh:class    occ:Occupant ;
    owl:inverseOf   occ:hasAccessTo ;
.

occ:Clo
  a qudt:Unit ;
  dcterms:description "A clo (clothing insulation) is a measure of the thermal insulation provided by clothing. 1 clo is defined as the amount of insulation that allows a person at rest to maintain thermal equilibrium in an environment at 21 degrees Celsius in a normally ventilated room (0.1 m/s air movement)."^^qudt:LatexString ;
  qudt:dbpediaMatch "https://dbpedia.org/page/Thermal_insulation"^^xsd:anyURI ;
  qudt:hasDimensionVector qkdv:A0E0L0I0M0H0T0D1 ;
  qudt:hasQuantityKind quantitykind:Dimensionless ;
  qudt:informativeReference "https://en.wikipedia.org/wiki/Clothing_insulation"^^xsd:anyURI ;
  qudt:symbol "clo" ;
  rdfs:isDefinedBy <http://qudt.org/2.1/vocab/unit> ;
  rdfs:label "clo"@en ;
.
