@prefix brick: <https://brickschema.org/schema/1.1/Brick#> .
@prefix occ: <https://brickschema.org/schema/1.1/Brick/extension/occupancy#> .
@prefix owl: <http://www.w3.org/2002/07/owl#> .
@prefix qudt: <http://qudt.org/schema/qudt/> .
@prefix rdf: <http://www.w3.org/1999/02/22-rdf-syntax-ns#> .
@prefix rdfs: <http://www.w3.org/2000/01/rdf-schema#> .
@prefix skos: <http://www.w3.org/2004/02/skos/core#> .

occ:Adjustable a occ:OccupantAccessibilityLevel ;
    skos:definition "Device is accessible to occupants" .

occ:Age a brick:Quantity .

occ:AgeRange a brick:Quantity ;
    owl:oneOf ( occ:AgeRange_Children occ:AgeRange_Teens occ:AgeRange_Adults occ:AgeRange_Elderly occ:AgeRange_Children occ:AgeRange_Teens occ:AgeRange_Adults occ:AgeRange_Elderly ) .

occ:AutomaticMode a occ:ModeOfControl ;
    skos:definition "Device is controlled automatically, according to some schedule" .

occ:ContinuousControl a occ:DegreeOfControl ;
    skos:definition "Device supports a continuous range of control inputs (e.g. 0-100%)" .

occ:DynamicMode a occ:ModeOfControl ;
    skos:definition "Device is controlled by a dynamic process, e.g. via a grid signal" .

occ:Gender a brick:Quantity ;
    owl:oneOf ( occ:Gender_Male occ:Gender_Female occ:Gender_Non-binary occ:Gender_Decline_to_state ) .

occ:ManualMode a occ:ModeOfControl ;
    skos:definition "Device is controlled manually" .

occ:NoControl a occ:DegreeOfControl ;
    skos:definition "Device is fixed or has no control input capabilities" .

occ:NotAccessible a occ:OccupantAccessibilityLevel ;
    skos:definition "Device is inaccessible to occupants" .

occ:OnOffControl a occ:DegreeOfControl ;
    skos:definition "Device has on/off binary control" .

occ:Permenance a brick:Quantity ;
    owl:oneOf ( occ:Permenance_Temporary occ:Permenance_Regular ) .

occ:Regular_Occupant a owl:Class ;
    rdfs:label "Regular Occupant" ;
    rdfs:subClassOf occ:Occupant ;
    skos:definition "A regular building occupant; e.g. an employee" .

occ:Shared a occ:OccupantAccessibilityLevel ;
    skos:definition "Device is accessible by many occupants" .

occ:StagedControl a occ:DegreeOfControl ;
    skos:definition "Device has a fixed number (> 2) of inputs" .

occ:Temporary_Occupant a owl:Class ;
    rdfs:label "Temporary Occupant" ;
    rdfs:subClassOf occ:Occupant ;
    skos:definition "A temporary building occupant; e.g. a visitor" .

occ:Window a owl:Class ;
    rdfs:label "Window" ;
    rdfs:subClassOf occ:Envelope_Equipment ;
    skos:definition "An opening in the wall or roof of a building or vehicle that is fitted with glass or other transparent material in a frame to admit light or air and allow people to see out." .

occ:Envelope_Equipment a owl:Class ;
    rdfs:label "Envelope Equipment" ;
    rdfs:subClassOf brick:Equipment ;
    skos:definition "Equipment used in the building envelope" .

occ:Gender_Decline_to_state a qudt:Quantity .

occ:Gender_Female a qudt:Quantity .

occ:Gender_Male a qudt:Quantity .

occ:Gender_Non-binary a qudt:Quantity .

occ:Permenance_Regular a qudt:Quantity ;
    skos:definition "A regular building occupant; e.g. an employee" .

occ:Permenance_Temporary a qudt:Quantity ;
    skos:definition "A temporary building occupant; e.g. a visitor" .

occ:AgeRange_Adults a qudt:Quantity ;
    skos:definition "Occupants are between 18 to 64 years old (inclusive)" .

occ:AgeRange_Children a qudt:Quantity ;
    skos:definition "Occupants are less than 11 years old (inclusive)" .

occ:AgeRange_Elderly a qudt:Quantity ;
    skos:definition "Occupants are more than 65 years old (inclusive)" .

occ:AgeRange_Teens a qudt:Quantity ;
    skos:definition "Occupants are between 12 to 17 years old (inclusive)" .

occ:Occupant a owl:Class ;
    rdfs:label "Occupant" ;
    rdfs:subClassOf brick:Class ;
    skos:definition "A building occupant" .

occ:DeviceProperty a owl:Class ;
    rdfs:label "DeviceProperty" ;
    rdfs:subClassOf brick:Class ;
    skos:definition "Properties of devices that relate to occupants and their interactions with devices" .

occ:ModeOfControl a owl:Class ;
    rdfs:label "ModeOfControl" ;
    rdfs:subClassOf occ:DeviceProperty ;
    skos:definition "The policy under which the device is controlled" .

occ:OccupantAccessibilityLevel a owl:Class ;
    rdfs:label "OccupantAccessibilityLevel" ;
    rdfs:subClassOf occ:DeviceProperty ;
    skos:definition "How accessible a device is to be controlled by occupants" .

occ:DegreeOfControl a owl:Class ;
    rdfs:label "DegreeOfControl" ;
    rdfs:subClassOf occ:DeviceProperty ;
    skos:definition "How a device may be controlled by an occupant" .
