@prefix brick: <https://brickschema.org/schema/Brick#> .
@prefix occ: <https://brickschema.org/schema/Brick/extension/occupancy#> .
@prefix owl: <http://www.w3.org/2002/07/owl#> .
@prefix qudt: <http://qudt.org/schema/qudt/> .
@prefix rdf: <http://www.w3.org/1999/02/22-rdf-syntax-ns#> .
@prefix rdfs: <http://www.w3.org/2000/01/rdf-schema#> .
@prefix skos: <http://www.w3.org/2004/02/skos/core#> .

occ:Adjustable a occ:OccupantAccessibilityLevel ;
    skos:definition "Device is accessible to occupants for adjustment" .

occ:Age a brick:Quantity .

occ:AgeRange a brick:Quantity ;
    owl:oneOf ( occ:AgeRange_Children occ:AgeRange_Teens occ:AgeRange_Adults occ:AgeRange_Elderly occ:AgeRange_Children occ:AgeRange_Teens occ:AgeRange_Adults occ:AgeRange_Elderly ) .

occ:AutomaticMode a occ:ModeOfControl ;
    skos:definition "Device is controlled automatically, according to some schedule" .

occ:Ceiling_Fan a owl:Class ;
    rdfs:label "Ceiling Fan" ;
    rdfs:subClassOf occ:Personal_Device ;
    skos:definition "A mechanical fan mounted on the ceiling of a room or space, usually electrically powered, that uses hub-mounted rotating blades to circulate air" .

occ:ContinuousControl a occ:DegreeOfControl ;
    skos:definition "Device supports a continuous range of control inputs (e.g. 0-100%)" .

occ:Desktop_Light a owl:Class ;
    rdfs:label "Desktop Light" ;
    rdfs:subClassOf occ:Personal_Device ;
    skos:definition "A lighting equipment on the desktop to provide illuminance" .

occ:Door a owl:Class ;
    rdfs:label "Door" ;
    rdfs:subClassOf occ:Envelope_Equipment ;
    skos:definition "A hinged, sliding, or revolving barrier at the entrance of a building or a zone that allows occupants to go in and out" .

occ:Door_Status a owl:Class ;
    rdfs:label "Door Status" ;
    rdfs:subClassOf occ:Status ;
    skos:definition "Status of the doors (open, closed)" .

occ:DynamicMode a occ:ModeOfControl ;
    skos:definition "Device is controlled by a dynamic process, e.g. via a grid signal" .

occ:Energy_Use_Style a brick:Quantity ;
    owl:oneOf ( occ:Energy_Use_Style_Austerity occ:Energy_Use_Style_Wasteful occ:Energy_Use_Style_Norm ) .

occ:Gender a brick:Quantity ;
    owl:oneOf ( occ:Gender_Male occ:Gender_Female occ:Gender_Nonbinary occ:Gender_Decline_to_state ) .

occ:Lighting_Status a owl:Class ;
    rdfs:label "Lighting Status" ;
    rdfs:subClassOf occ:Status ;
    skos:definition "Status of the lightings (on, off)" .

occ:ManualMode a occ:ModeOfControl ;
    skos:definition "Device is controlled manually" .

occ:NoControl a occ:DegreeOfControl ;
    skos:definition "Device is fixed or has no control input capabilities" .

occ:NotAccessible a occ:OccupantAccessibilityLevel ;
    skos:definition "Device is inaccessible to occupants" .

occ:OnOffControl a occ:DegreeOfControl ;
    skos:definition "Device has on/off binary control" .

occ:Permenance a brick:Quantity ;
    owl:oneOf ( occ:Permenance_Individual occ:Permenance_Group ) .

occ:Portable_Fan a owl:Class ;
    rdfs:label "Portable Fan" ;
    rdfs:subClassOf occ:Personal_Device ;
    skos:definition "A cord-connected appliance that is easily moved by hand from place to place to provide flowing air" .

occ:Portable_Heater a owl:Class ;
    rdfs:label "Portable Heater" ;
    rdfs:subClassOf occ:Personal_Device ;
    skos:definition "A cord-connected appliance that is easily moved by hand from place to place to provide heating" .

occ:Race a brick:Quantity ;
    owl:oneOf ( occ:Race_African_American occ:Race_Asian occ:Race_American_Indian occ:Race_Native_Hawaiian occ:Race_White occ:Race_Mix ) .

occ:Regular_Occupant a owl:Class ;
    rdfs:label "Regular Occupant" ;
    rdfs:subClassOf occ:Occupant ;
    skos:definition "A regular building occupant; e.g. an employee" .

occ:Shading_Sensor a owl:Class ;
    rdfs:label "Shading Sensor" ;
    rdfs:subClassOf occ:Sensor ;
    skos:definition "A sensor used to monitor the status of the shading (on, off)" .

occ:Shared a occ:OccupantAccessibilityLevel ;
    skos:definition "Device is accessible by multiple occupants" .

occ:StagedControl a occ:DegreeOfControl ;
    skos:definition "Device has a fixed number (> 2) of inputs" .

occ:Temporary_Occupant a owl:Class ;
    rdfs:label "Temporary Occupant" ;
    rdfs:subClassOf occ:Occupant ;
    skos:definition "A temporary building occupant; e.g. a visitor" .

occ:Thermal_Preference a brick:Quantity ;
    owl:oneOf ( occ:Thermal_Preference_Warmer occ:Thermal_Preference_Cooler occ:Thermal_Preference_Neutral occ:Thermal_Preference_No_Preference ) .

occ:Wifi_AP a owl:Class ;
    rdfs:label "Wifi AP" ;
    rdfs:subClassOf occ:Sensor ;
    skos:definition "Number of wifi access point" .

occ:Window a owl:Class ;
    rdfs:label "Window" ;
    rdfs:subClassOf occ:Envelope_Equipment ;
    skos:definition "An opening in the wall of a building to admit light or air and allows occupants to see out" .

occ:Window_Sensor a owl:Class ;
    rdfs:label "Window Sensor" ;
    rdfs:subClassOf occ:Sensor ;
    skos:definition "A sensor used to monitor the status of the window (open, closed, open angle)" .

occ:Window_Status a owl:Class ;
    rdfs:label "Window Status" ;
    rdfs:subClassOf occ:Status ;
    skos:definition "Status of the windows (open, closed)" .

occ:Energy_Use_Style_Austerity a qudt:Quantity ;
    skos:definition "Occupants have an austerity energy use behavior" .

occ:Energy_Use_Style_Norm a qudt:Quantity ;
    skos:definition "Occupants have an average energy use behavior" .

occ:Energy_Use_Style_Wasteful a qudt:Quantity ;
    skos:definition "Occupants have a wasteful energy use behavior" .

occ:Gender_Decline_to_state a qudt:Quantity ;
    skos:definition "Occupants declined to state" .

occ:Gender_Female a qudt:Quantity ;
    skos:definition "Occupants are female" .

occ:Gender_Male a qudt:Quantity ;
    skos:definition "Occupants are male" .

occ:Gender_Nonbinary a qudt:Quantity ;
    skos:definition "Occupants are non-binary" .

occ:Permenance_Group a qudt:Quantity ;
    skos:definition "A description of a certain group of occupant" .

occ:Permenance_Individual a qudt:Quantity ;
    skos:definition "A description of one individual occupant" .

occ:Race_African_American a qudt:Quantity ;
    skos:definition "Occupants are African American" .

occ:Race_American_Indian a qudt:Quantity ;
    skos:definition "Occupants are American Indian" .

occ:Race_Asian a qudt:Quantity ;
    skos:definition "Occupants are Asian" .

occ:Race_Mix a qudt:Quantity ;
    skos:definition "The group of occupants has a mix of races" .

occ:Race_Native_Hawaiian a qudt:Quantity ;
    skos:definition "Occupants are Native Hawaiian" .

occ:Race_White a qudt:Quantity ;
    skos:definition "Occupants are white people" .

occ:Thermal_Preference_Cooler a qudt:Quantity ;
    skos:definition "Occupants prefer cooler indoor environment" .

occ:Thermal_Preference_Neutral a qudt:Quantity ;
    skos:definition "Occupants prefer neutral indoor environment" .

occ:Thermal_Preference_No_Preference a qudt:Quantity ;
    skos:definition "Occupants do not have special thermal preference" .

occ:Thermal_Preference_Warmer a qudt:Quantity ;
    skos:definition "Occupants prefer warmer indoor environment" .

occ:AgeRange_Adults a qudt:Quantity ;
    skos:definition "Occupants are between 18 to 64 years old (inclusive)" .

occ:AgeRange_Children a qudt:Quantity ;
    skos:definition "Occupants are less than 11 years old (inclusive)" .

occ:AgeRange_Elderly a qudt:Quantity ;
    skos:definition "Occupants are more than 65 years old (inclusive)" .

occ:AgeRange_Teens a qudt:Quantity ;
    skos:definition "Occupants are between 12 to 17 years old (inclusive)" .

occ:Envelope_Equipment a owl:Class ;
    rdfs:label "Envelope Equipment" ;
    rdfs:subClassOf brick:Equipment ;
    skos:definition "Equipment used in the building envelope" .

occ:Occupant a owl:Class ;
    rdfs:label "Occupant" ;
    rdfs:subClassOf brick:Class ;
    skos:definition "Building occupant, which can be an indiviudal occupant or a group of occupants sharing some common attributes" .

occ:DeviceProperty a owl:Class ;
    rdfs:label "DeviceProperty" ;
    rdfs:subClassOf brick:Class ;
    skos:definition "Properties of devices that relate to occupants and their interactions with devices" .

occ:ModeOfControl a owl:Class ;
    rdfs:label "ModeOfControl" ;
    rdfs:subClassOf occ:DeviceProperty ;
    skos:definition "The policy under which the device is controlled" .

occ:OccupantAccessibilityLevel a owl:Class ;
    rdfs:label "OccupantAccessibilityLevel" ;
    rdfs:subClassOf occ:DeviceProperty ;
    skos:definition "How accessible a device is to be controlled by occupants" .

occ:Sensor a owl:Class ;
    rdfs:label "Sensor" ;
    rdfs:subClassOf brick:Status ;
    skos:definition "A Sensor is an input point that represents the value of a device or instrument designed to detect and measure a variable (ASHRAE Dictionary)" .

occ:Status a owl:Class ;
    rdfs:label "Status" ;
    rdfs:subClassOf brick:Status ;
    skos:definition "Status of the equipment" .

occ:DegreeOfControl a owl:Class ;
    rdfs:label "DegreeOfControl" ;
    rdfs:subClassOf occ:DeviceProperty ;
    skos:definition "How a device may be controlled by an occupant" .

occ:Personal_Device a owl:Class ;
    rdfs:label "Personal Device" ;
    rdfs:subClassOf brick:Equipment ;
    skos:definition "Dedicated devices used to maintain thermal comfort for occupants" .
