@prefix brick: <https://brickschema.org/schema/Brick#> .
@prefix occ: <https://brickschema.org/schema/Brick/extension/occupancy#> .
@prefix sh: <http://www.w3.org/ns/shacl#> .
@prefix owl: <http://www.w3.org/2002/07/owl#> .
@prefix rdf: <http://www.w3.org/1999/02/22-rdf-syntax-ns#> .
@prefix rdfs: <http://www.w3.org/2000/01/rdf-schema#> .
@prefix skos: <http://www.w3.org/2004/02/skos/core#> .
@prefix foaf: <http://xmlns.com/foaf/0.1/> .
@prefix sdo: <http://schema.org/> .
@prefix dcterms: <http://purl.org/dc/terms#> .
@prefix unit: <http://qudt.org/vocab/unit/> .
@prefix xsd: <http://www.w3.org/2001/XMLSchema#> .


########## Occupant Classes

occ:Occupant a owl:Class ;
    rdfs:label "Occupant" ;
    rdfs:subClassOf  brick:Entity, foaf:Agent ;
    skos:definition "Building occupant, which can be an individual occupant or a group of occupants sharing some common attributes" .

occ:Group   a   owl:Class, sh:NodeShape ;
    sh:property [
        sh:path occ:label ;
        sh:minCount 1 ;
    ] ;
    rdfs:subClassOf foaf:Group, occ:Occupant ;
    skos:definition "One or more building occupants or groups" ;
.

occ:Individual   a   owl:Class, sh:NodeShape ;
    sh:property [
        sh:path occ:label ;
        sh:minCount 1 ;
    ] ;
    rdfs:subClassOf foaf:Person, occ:Occupant ;
    skos:definition "A single building occupant" ;
.

################# Properties

occ:groupSize    a   owl:DatatypeProperty ;
    rdfs:domain occ:Group ;
    rdfs:range  xsd:positiveInteger ;
    skos:definition "The number of individuals in a group" ;
.

occ:hasMember   a   owl:ObjectProperty ;
    owl:inverseOf occ:isMemberOf ;
    rdfs:domain occ:Group ;
    rdfs:range occ:Occupant ;
.

occ:isMemberOf   a   owl:ObjectProperty ;
    owl:inverseOf occ:hasMember ;
    rdfs:domain occ:Occupant ;
    rdfs:range occ:Group ;
.

occ:ethnicity  a   owl:ObjectProperty;
    rdfs:domain occ:Individual ;
    sh:in   ("American Indian or Alaska Native"
             "Asian or Asian American"
             "Black or African American"
             "Hispanic, Latino, Latina, or Latinx"
             "Middle Eastern or Northern African"
             "Native Hawaiian or Other Pacific Islander"
             "White"
             "An ethnicity not listed here"
             "Decline to state") ;
.


occ:age a   brick:EntityProperty ;
    rdfs:domain occ:Occupant ;
    skos:definition "The age or age range of the occupant" ;
.

occ:clothingInsulation a   brick:EntityProperty ;
    skos:definition "The range or value of I_cl clothing insulation values that the occupant is wearing" ;
    rdfs:domain occ:Occupant ;
.

occ:gender  a   owl:ObjectProperty;
    rdfs:domain occ:Occupant ;
    sh:in   ("Male" "Female" "Transgender" "A gender not listed here" "Decline to state") ;
    # second question from https://gender.stanford.edu/news-publications/gender-news/more-inclusive-gender-questions-added-general-social-survey
.

occ:clothingInsulationRange a   owl:ObjectProperty ;
    skos:definition "The range or value of insulation of the clothing worn by an occupant, measured in Clo" ;
    rdfs:domain occ:Occupant ;
    rdfs:range  occ:ClothingInsulationRange ;
.

occ:clothingDescription a   owl:DatatypeProperty ;
    skos:definition "A description of the clothing worn by an occupant; should be used to derive a Clo value or range (see occ:clothingInsulationRange)" ;
    rdfs:domain occ:Occupant ;
    rdfs:range  xsd:string ;
.

occ:thermalComfortPreference a owl:ObjectProperty ;
    rdfs:range  occ:ThermalComfortPreference ;
.
